Some improvements and updated examples

examples/ResourceManager.thy
@@ -1,49 +1,49 @@
+section \<open> Resource Manager \<close>
+
 theory ResourceManager
-  imports "Interaction_Trees.ITree_Simulation"
+  imports "Interaction_Trees.ITree_Simulation" "Interaction_Trees.ITree_Machine"
 begin 
 
 unbundle Circus_Syntax
 
 lit_vars
 
+consts RES :: "integer set"
+
 schema ResourceManager =
   res  :: "integer set"
   free :: "integer set"
-  where "free \<subseteq> res"
+  where "free \<subseteq> res" "res \<subseteq> RES"
 
 record_default ResourceManager
 
-chantype chan =
-  alloc :: integer
-  dealloc :: integer
+zoperation Allocate =
+  over ResourceManager
+  params r \<in> RES
+  pre "r \<in> free"
+  update "[free \<leadsto> free - {r}]"
 
-definition Allocate :: "(chan, ResourceManager) htree" where
-"Allocate = alloc?(r):free \<rightarrow> free := free - {r}"
+zoperation Allocate\<^sub>1 =
+  over ResourceManager
+  params r \<in> RES
+  pre "r \<in> free \<and> r = Min free"
+  update "[free \<leadsto> free - {r}]"
 
-term "operation alloc (\<lambda> r. (r \<in> free) & free := free - {r})"
+zoperation Deallocate =
+  over ResourceManager
+  params r \<in> RES
+  pre "r \<notin> free"
+  update "[free \<leadsto> free \<union> {r}]"
 
-text \<open> If we just select the minimum of free, the simulation crashes when all resources are allocated. 
-  Adding the intersection with @{const free} means that @{term "(Min free)\<^sub>e"} is not evaluated due
-  to lazy evaluation in Haskell. \<close>
+lemma Allocate\<^sub>1_refines_Allocate: "Allocate r \<sqsubseteq> Allocate\<^sub>1 r"
+  apply (simp add: Allocate_def Allocate\<^sub>1_def input_in_rel assigns_rel refined_by_def input_in_pre assigns_pre seq_pre wp mk_zop_def)
+  oops
 
-definition Allocate\<^sub>1 :: "(chan, ResourceManager) htree" where
-"Allocate\<^sub>1 = alloc?(r):(free \<inter> {Min free}) \<rightarrow> free := free - {r}"
+zmachine ResourceManagerProc =
+  init "[res \<leadsto> RES, free \<leadsto> RES]"
+  operations "Allocate" "Deallocate"
 
-lemma Allocate\<^sub>1_refines_Allocate: "Allocate \<sqsubseteq> Allocate\<^sub>1"
-  by (simp add: Allocate_def Allocate\<^sub>1_def input_in_rel assigns_rel refined_by_def input_in_pre assigns_pre)
-     (expr_auto)
-
-definition Deallocate :: "(chan, ResourceManager) htree" where
-"Deallocate = dealloc?(r):(res - free) \<rightarrow> free := free \<union> {r}"
-
-consts RES :: "integer list"
-
-definition "ResourceManagerProc
-  = process [res \<leadsto> set RES, free \<leadsto> set RES] (loop (Allocate \<box> Deallocate))"
-
-term integer_of_int
-
-def_consts RES = "map integer_of_int [0..5]"
+def_consts RES = "set (map integer_of_int [0..5])"
 
 simulate ResourceManagerProc
 
